Weidenbach_Book/IsaSAT_Initialisation.thy
@@ -2288,6 +2288,8 @@ proof -
     apply (auto simp: uint32_max_def)
     apply (auto simp: max_def  \<L>\<^sub>a\<^sub>l\<^sub>l_add_mset)
     done
+
+
   show ?thesis
     apply (intro frefI nres_relI)
     subgoal for x y
